more work on the reduction

theories/L/Complexity/Problems/LGraph.v
@@ -2,7 +2,7 @@ From Undecidability.L Require Export L.
 From Undecidability.L.Tactics Require Import LTactics GenEncode.
 From Undecidability.L.Datatypes Require Export Lists.
 Require Import PslBase.FiniteTypes. 
-From Undecidability.L.Complexity Require Export ONotation Monotonic. 
+From Undecidability.L.Complexity Require Export ONotation Monotonic MorePrelim.
 
 (* for the L representation, the symmetric closure is implicit
  (i.e. we do not require the edge list to contain symmetric edges)*)
@@ -45,23 +45,6 @@ Proof.
 Qed. 
 
 (* deciders for node and edge containment*)
-
-Section pair_eq.
-  Variable (X Y : Type). 
-  Variable  (eqbX : X -> X -> bool) (eqbY : Y -> Y -> bool). 
-  Variable (eqbX_correct : forall a b, a = b <-> eqbX a b = true).
-  Variable (eqbY_correct : forall a b, a = b <-> eqbY a b = true).
-
-  Definition pair_eqb (a b : (X * Y)%type) : bool :=
-    match a, b with (x1, y1), (x2, y2) => eqbX x1 x2 && eqbY y1 y2 end. 
-
-  Lemma pair_eqb_correct a b : a = b <-> pair_eqb a b = true.
-  Proof.
-    destruct a, b. split. 
-    + intros H. cbn. apply andb_true_intro; split.
-      apply eqbX_correct; congruence. apply eqbY_correct; congruence. 
-    + intros [H1 H2]%andb_prop. apply eqbX_correct in H1. apply eqbY_correct in H2. congruence. Qed. 
-End pair_eq. 
 
 
 Definition Lgraph_node_in_dec (g : Lgraph) (node : Lnode) := match g with (max, _) => Nat.leb (S node) max end. 
