theories/L/Complexity/MorePrelim.v
@@ -1,0 +1,19 @@
+Require Import PslBase.Base.
+
+Section pair_eq.
+  Variable (X Y : Type). 
+  Variable  (eqbX : X -> X -> bool) (eqbY : Y -> Y -> bool). 
+  Variable (eqbX_correct : forall a b, a = b <-> eqbX a b = true).
+  Variable (eqbY_correct : forall a b, a = b <-> eqbY a b = true).
+
+  Definition pair_eqb (a b : (X * Y)%type) : bool :=
+    match a, b with (x1, y1), (x2, y2) => eqbX x1 x2 && eqbY y1 y2 end. 
+
+  Lemma pair_eqb_correct a b : a = b <-> pair_eqb a b = true.
+  Proof.
+    destruct a, b. split. 
+    + intros H. cbn. apply andb_true_intro; split.
+      apply eqbX_correct; congruence. apply eqbY_correct; congruence. 
+    + intros [H1 H2]%andb_prop. apply eqbX_correct in H1. apply eqbY_correct in H2. congruence. Qed. 
+End pair_eq. 
+
